Pattern: Implement simultanous substitutions

LeanChecker/Pattern.lean
@@ -12,26 +12,30 @@ def ph1 : Pattern := (Pattern.metavar 1)
 def ph2 : Pattern := (Pattern.metavar 2)
 def ph0_implies_ph0 : Pattern := (implies ph0 ph0)
 
-def Pattern.instantiate(p: Pattern)(subst: Nat × Pattern) : Pattern :=
-    match subst with | (id, plug) => match p with
-      | Pattern.metavar id' => if id' = id then plug else p
+def Pattern.instantiate(p: Pattern)(subst: List (Nat × Pattern)) : Pattern :=
+    match p with
+      | Pattern.metavar id' =>
+            match subst with
+             | [] => p
+             | (id, plug) :: rest
+                => if id' = id then plug else p.instantiate rest
       | Pattern.bot => Pattern.bot
-      | Pattern.implies left right => Pattern.implies (instantiate left (id, plug)) (instantiate right (id, plug))
+      | Pattern.implies left right => Pattern.implies (left.instantiate subst) (right.instantiate subst)
 
 theorem test_inst_1 :
-    (Pattern.instantiate Pattern.bot (0, ph0)) = Pattern.bot := by rfl
+    (Pattern.instantiate Pattern.bot [(0, ph0)]) = Pattern.bot := by rfl
 theorem test_inst_2 :
-    (Pattern.instantiate ph0 (0, ph0)) = ph0 := by rfl
+    (Pattern.instantiate ph0 [(0, ph0)]) = ph0 := by rfl
 theorem test_inst_3 :
-    (Pattern.instantiate ph1 (0, ph0)) = ph1 := by rfl
+    (Pattern.instantiate ph1 [(0, ph0)]) = ph1 := by rfl
 theorem test_inst_4 :
-    (Pattern.instantiate ph0_implies_ph0 (0, ph1)) = (implies ph1 ph1) := by rfl
+    (Pattern.instantiate ph0_implies_ph0 [(0, ph1)]) = (implies ph1 ph1) := by rfl
 theorem test_inst_5 :
-    (Pattern.instantiate ph0_implies_ph0 (0, ph0_implies_ph0)) = (implies ph0_implies_ph0 ph0_implies_ph0) := by rfl
+    (Pattern.instantiate ph0_implies_ph0 [(0, ph0_implies_ph0)]) = (implies ph0_implies_ph0 ph0_implies_ph0) := by rfl
 
 
 inductive Proof where
-    | instantiate(schema: Proof)(id: Nat)(value: Pattern) : Proof /-- TODO: We need simultanous substitutions here --/
+    | instantiate(schema: Proof)(subst: List (Nat × Pattern)) : Proof /-- TODO: We need simultanous substitutions here --/
     | prop1 : Proof
     | prop2 : Proof
     | modus_ponens(left: Proof)(right: Proof) : Proof
@@ -43,10 +47,10 @@ def mp := Proof.modus_ponens
 
 def Proof.conclusion(pi: Proof) : Option Pattern :=
     match pi with
-      | Proof.instantiate pi' id' plug' =>
+      | Proof.instantiate pi' subst' =>
         match pi'.conclusion with
           | none => none
-          | some concl' => (concl'.instantiate (id', plug'))
+          | some concl' => (concl'.instantiate subst')
       | Proof.prop1 => (implies ph0 (implies ph1 ph0))
       | Proof.prop2 => (implies (implies ph0 (implies ph1 ph2)) (implies (implies ph0  ph1) (implies ph0 ph2)))
       | Proof.modus_ponens pi1 pi2 =>
@@ -58,11 +62,10 @@ def Proof.conclusion(pi: Proof) : Option Pattern :=
           | (some _, some _) => none
 
 def imp_refl: Proof :=
-    (mp (mp (inst (inst prop2 1 ph0_implies_ph0)
-                              2 ph0)
-            (inst prop1 1 ph0_implies_ph0)
+    (mp (mp (inst prop2 [(1, ph0_implies_ph0), (2, ph0)])
+            (inst prop1 [(1, ph0_implies_ph0)])
         )
-        (inst prop1 1 ph0)
+        (inst prop1 [(1, ph0)])
     )
 
 theorem test_imp_refl : imp_refl.conclusion = some ph0_implies_ph0 := by rfl
